\subsection{Solving Recurrence Relations with Induction}

\subsubsection{Example}
\textbf{Prove that the following systems of equations has the solution $T(n) = n \cdot lg(n)$.}
$$
T(n) \begin{cases}
	2T(\frac{n}{2}) + n, & n = 2^k \mbox{ for } k > 1\\
	2, & n = 2
\end{cases}
$$
\textbf{Basis}
\begin{eqnarray*}
T(2) &=& (2) \cdot lg(2)\\
	&=& 2 \cdot 1\\
	&=& 2
\end{eqnarray*}
\textbf{Inductive Hypothesis}\\
Assume that $T(n) = n \cdot lg(n)$ holds true for all $n = 2^k$.\\\\
\textbf{Inductive Step}
\begin{align*}
T(n)	&=	2T(\frac{n}{2}) + n						&& \text{Base equation}\\
		&= 	2T(\frac{2^{k+1}}{2}) + 2^{k+1}			&& \text{Substitute n with } 2^{k+1}\\
		&= 	2T(2^{k}) + 2^{k+1}						&& \text{Simplify parameters to function T(...)}\\
		&=	2(2^k \cdot lg(2^k)) + 2^{k+1}			&& \text{Inductive hypothesis}\\
		&=	2^{k+1} \left[ lg(2^k) + 1 \right]		&& \text{Distributive property}\\
		&=  2^{k+1} \left[ lg(2^k) + lg(2) \right]  && \text{Logarithmic identity}\\
		&= 	2^{k+1} \cdot lg(2^k \cdot 2)			&& \text{Logarithmic identity}\\
		&=  2^{k+1} \cdot lg(2^{k+1})				&& \text{Exponent property}\\
		&											&& \text{Q.E.D}
\end{align*}

\subsubsection{Example}
\textbf{Prove that the following systems of equations has the solution $T(n) = 2F(n) - 1$ where $F(n) = F(n-1) + F(n-2)$.}
$$
T(n) \begin{cases}
T(n-1) + T(n-2) + 1, & \mbox{if } n \geq 2\\
0, & \mbox{if } n = \{0,1\}
\end{cases}
$$
\textbf{Basis}
\begin{eqnarray*}
	T(0) &=& 1
\end{eqnarray*}
\textbf{Inductive Hypothesis}\\
Assume that $T(n) = F(n) - 1$ is true for all $n = k$.\\
\textbf{Inductive Step}
\begin{align*}
	T(n) 	&= T(n-1) + T(n-2) + 1					&& \text{Base equation}\\
	T(k+1) 	&= T((k+1) - 1) + T((k+1) - 2) + 1 		&& \text{Substitute n with k+1}\\
			&= T(k) + T(k-1) + 1					&& \text{Simplify parameters to function T(...)}\\
			&= (2F(k) - 1) + (2F(k-1) - 1) + 1		&& \text{Inductive hypothesis}\\
			&= 2F(k) + 2F(k-1) - 1					&& \text{Simplify equation}\\
			&= 2(F(k) + F(k-1)) - 1					&& \text{Distributive property}\\
			&= 2(F(k+1)) - 1						&& \text{Definition of function: } F(k+1) = F(k) + F(k-1)\\
			&= 2F(k+1) - 1							&& \text{Simplify}\\
			&										&& \text{Q.E.D}
\end{align*}